DeBruijnSSA/BinSyntax/Rewrite/Region/Compose/Elgot.lean
@@ -39,12 +39,76 @@ def Eqv.control {A B : Ty α} {Γ : Ctx α ε} {L : LCtx α}
     (br 1 (var 0 (by simp)) ⟨by simp, le_refl _⟩)
     (ret (var 0 (by simp)))
 
+@[simp]
+theorem Eqv.vwk1_control {A B : Ty α} {Γ : Ctx α ε} {L : LCtx α}
+  : (control (φ := φ) (A := A) (B := B) (Γ := Γ) (L := L)).vwk1 (inserted := inserted) = control
+  := rfl
+
+@[simp]
+theorem Eqv.vwk2_control {A B : Ty α} {Γ : Ctx α ε} {L : LCtx α}
+  : (control (φ := φ) (A := A) (B := B) (Γ := (X::Γ)) (L := L)).vwk2 (inserted := inserted)
+  = control
+  := rfl
+
 def Eqv.fixpoint {A B : Ty α} {Γ : Ctx α ε} {L : LCtx α} (f : Eqv φ (⟨A, ⊥⟩::Γ) ((B.coprod A)::L))
   : Eqv φ (⟨A, ⊥⟩::Γ) (B::L) := cfg [A] nil (λ| ⟨0, _⟩ => f.vwk1.lwk1 ;; control)
 
+theorem Eqv.fixpoint_iter_cfg {A B : Ty α} {Γ : Ctx α ε} {L : LCtx α}
+  (f : Eqv φ (⟨A, ⊥⟩::Γ) ((B.coprod A)::L))
+  : fixpoint f = cfg [A] (f.lwk1 ;; control) (λ| ⟨0, _⟩ => f.vwk1.lwk1 ;; control) := by
+  rw [fixpoint, <-ret_nil, ret, cfg_br_lt (hℓ' := by simp)]
+  congr
+  simp only [List.singleton_append, List.length_singleton, Nat.zero_eq, Fin.zero_eta, Fin.isValue,
+    List.get_eq_getElem, Fin.val_zero, List.getElem_cons_zero, List.append_eq, List.nil_append,
+    vwk_id_eq, let1_beta]
+  rw [lwk1_vwk1, seq, vsubst_lsubst, seq]
+  congr
+  . rw [vsubst_alpha0]
+    rfl
+  . induction f using Quotient.inductionOn
+    simp only [Term.Eqv.nil, var, subst0_quot, lwk1_quot, vwk1_quot, vsubst_quot]
+    apply congrArg
+    ext
+    simp only [Set.mem_setOf_eq, InS.coe_vsubst, Term.InS.coe_subst0, Term.InS.coe_var,
+      InS.coe_vwk1]
+    rw [Region.vwk1, <-Region.vsubst_fromWk, Region.vsubst_vsubst]
+    apply Eq.trans _ (Region.vsubst_id _)
+    congr
+    funext k
+    cases k <;> rfl
+
+theorem Eqv.seq_cont {A B C : Ty α} {Γ : Ctx α ε} {L : LCtx α}
+  (f : Eqv φ (⟨A, ⊥⟩::Γ) (B::L)) (g : Eqv φ (⟨B, ⊥⟩::Γ) (C::D::L))
+  (h : Eqv φ (⟨C, ⊥⟩::Γ) (C::D::L))
+  : cfg [C] (f.lwk1 ;; g) (λ⟨0, _⟩ => h.vwk1) = f ;; cfg [C] g (λ⟨0, _⟩ => h.vwk1)
+  := sorry
+
+theorem Eqv.ret_var_zero_eq_nil_vwk1 {A : Ty α} {Γ : Ctx α ε} {L : LCtx α}
+  : ret (var 0 (by simp)) = (nil (φ := φ) (ty := A) (rest := Γ) (targets := L)).vwk1 (inserted := X)
+  := rfl
+
 theorem Eqv.fixpoint_iter {A B : Ty α} {Γ : Ctx α ε} {L : LCtx α}
   (f : Eqv φ (⟨A, ⊥⟩::Γ) ((B.coprod A)::L))
-  : fixpoint f = f ;; coprod nil (fixpoint f) := sorry
+  : fixpoint f = f ;; coprod nil (fixpoint f) := by
+  apply Eq.trans f.fixpoint_iter_cfg
+  rw [lwk1_vwk1, <-vwk1_control]
+  simp only [<-vwk1_seq (left := f.lwk1) (right := control)]
+  rw [seq_cont]
+  congr
+  conv =>
+    lhs
+    lhs
+    rw [control]
+  rw [cfg_case, cfg_br_ge (ℓ := 1) (hℓ' := by simp)]
+  simp only [List.length_singleton, Nat.sub_self, coprod]
+  congr
+  rw [fixpoint, vwk1_cfg]
+  congr
+  funext i
+  cases i using Fin.cases with
+  | zero =>
+    simp only [vwk1_seq, vwk1_control, vwk2_seq, vwk2_control, lwk1_vwk1, vwk1_vwk2]
+  | succ i => exact i.elim0
 
 theorem Eqv.fixpoint_naturality {A B C : Ty α} {Γ : Ctx α ε} {L : LCtx α}
   (f : Eqv φ (⟨A, ⊥⟩::Γ) ((B.coprod A)::L))
